Algorithm/Data/Graph.lean
@@ -1,26 +1,34 @@
 
 import Algorithm.Data.Classes.AssocArray
+import Algorithm.Data.Classes.Collection
 import Mathlib.Data.List.Nodup
 
 structure Graph where
-  V : Type _
+  V : Type*
   [decidableEqV : DecidableEq V]
-  EType : Type _
+  EType : Type*
+  [decidableEqEType : DecidableEq EType]
+  EColl : Type*
+  [collectionEColl : Collection EColl EType]
   fst' : EType → V
   snd' : EType → V
-  StarList : Type _
-  [assocArrayStarList : AssocArray StarList V (List EType)]
+  StarList : Type*
+  [inhabitedEColl : Inhabited EColl]
+  [assocArrayStarList : AssocArray StarList V EColl]
   star' : StarList
   costar' : StarList
-  fst_star' : ∀ v, ∀ e ∈ star'[v], fst' e = v
-  snd_costar' : ∀ v, ∀ e ∈ costar'[v], snd' e = v
-  nodup_star' : ∀ v : V, star'[v].Nodup
-  nodup_costar' : ∀ v : V, costar'[v].Nodup
-  mem_star'_iff_mem_costar' : ∀ e, e ∈ star'[fst' e] ↔ e ∈ costar'[snd' e]
+  fst_star' v : ∀ e ∈ star'[v], fst' e = v
+  snd_costar' v : ∀ e ∈ costar'[v], snd' e = v
+  count_star'_fst_eq_count_costar'_snd e :
+    Collection.count e star'[fst' e] = Collection.count e costar'[snd' e]
+  -- nodup_star' (v : V) : star'[v].Nodup
+  -- nodup_costar' (v : V) : costar'[v].Nodup
+  -- mem_star'_iff_mem_costar' e : e ∈ star'[fst' e] ↔ e ∈ costar'[snd' e]
 
 namespace Graph
 
-attribute [instance] decidableEqV assocArrayStarList
+attribute [instance] decidableEqV decidableEqEType collectionEColl inhabitedEColl
+  assocArrayStarList
 
 variable {g : Graph}
 -- instance : GetElem g.StarList g.V (List g.E) (fun _ _ ↦ True) := AssocArray.instGetElem
@@ -29,17 +37,22 @@ variable {g : Graph}
 def EType.fst (e : g.EType) : g.V := g.fst' e
 def EType.snd (e : g.EType) : g.V := g.snd' e
 
-def V.star (v : g.V) : List g.EType := g.star'[v]
-def V.costar (v : g.V) : List g.EType := g.costar'[v]
+def V.star (v : g.V) : g.EColl := g.star'[v]
+def V.costar (v : g.V) : g.EColl := g.costar'[v]
 
 lemma fst_star (v : g.V) : ∀ e ∈ v.star, e.fst = v := g.fst_star' v
 lemma snd_costar (v : g.V) : ∀ e ∈ v.costar, e.snd = v := g.snd_costar' v
 
-lemma nodup_star (v : g.V) : v.star.Nodup := g.nodup_star' v
-lemma nodup_costar (v : g.V) : v.costar.Nodup := g.nodup_costar' v
+lemma count_star_fst_eq_count_costar_snd (e : g.EType) :
+    Collection.count e e.fst.star = Collection.count e e.snd.costar :=
+  g.count_star'_fst_eq_count_costar'_snd e
 
-lemma mem_star_iff_mem_costar (e : g.EType) : e ∈ e.fst.star ↔ e ∈ e.snd.costar :=
-  g.mem_star'_iff_mem_costar' e
+-- lemma nodup_star (v : g.V) : v.star.Nodup := g.nodup_star' v
+-- lemma nodup_costar (v : g.V) : v.costar.Nodup := g.nodup_costar' v
+
+lemma mem_star_iff_mem_costar (e : g.EType) : e ∈ e.fst.star ↔ e ∈ e.snd.costar := by
+  rw [← Collection.count_ne_zero, ← Collection.count_ne_zero,
+    count_star_fst_eq_count_costar_snd]
 
 def E (g : Graph) := {e : g.EType // e ∈ e.fst.star}
 
